join and fix proof for all other queries

Relational2.v
@@ -1,10 +1,8 @@
 Require Import Bool Arith List CpdtTactics CorgiTactics.
 Set Implicit Arguments.
 
-Inductive tuple : Set :=
-  | TCons : nat -> tuple -> tuple
-  | TNil : tuple.
-
+Definition tuple : Set :=
+  list nat.
 
 Definition relation : Set :=
   list tuple.
@@ -23,7 +21,8 @@ Inductive Pred : Set :=
 Inductive Query : Set := 
   | Select : Bool -> Query
   | Project : nat -> Query
-  | SelectIf : Pred -> Query. (* overlaps with Select *)
+  | SelectIf : Pred -> Query(* overlaps with Select *)
+  | JoinFirst : Query. 
 (**
   end (Query language syntax)
 **)
@@ -31,9 +30,9 @@ Inductive Query : Set :=
 
 Fixpoint projectTuple (t: tuple) (index: nat) : option tuple :=
   match t with
-  | TNil => None
-  | TCons n rem => match index with
-                   | 0 => Some (TCons n TNil)
+  | nil => None
+  | n :: rem => match index with
+                   | 0 => Some (n :: nil)
                    | S index' => projectTuple rem index'
                    end
   end.
@@ -67,7 +66,7 @@ Fixpoint select (pr: Pred)  (input: relation) :=
     | PredFirst1 => match input with
                       | nil => nil
                       | t :: rem => match t with
-                                      | TCons 1 _ => t :: (select pr rem)
+                                      | 1 :: _ => t :: (select pr rem)
                                      (* picking semantics that length 0 tuples just fail the predicate rather than fail *)
                                       | _ => select pr rem
                                     end
@@ -83,17 +82,41 @@ match input with
     end.
 *)
 
-Eval simpl in project ((TCons 1 TNil) :: (TCons 2 TNil) :: nil) 0.
 
-Definition runQuery (q : Query) (inputRelation : relation) : option relation :=
+Definition joineq (t1 : tuple) (t2 : tuple) : bool :=
+  match t1, t2 with
+    | t1first :: _, t2first :: _ => beq_nat t1first t2first
+    | _, _ => false
+  end. 
+
+
+Fixpoint nljoin (r1 : relation) (r2 : relation) : relation :=
+  let fix nljoin_inner (t : tuple) (r : relation) : relation :=
+    match r with
+      | t' :: r' => if joineq t t' then (t ++ t') :: nljoin_inner t r' else nljoin_inner t r'
+      | nil => nil
+    end in
+
+  match r1 with
+    | t1 :: r1' => (nljoin_inner t1 r2) ++ nljoin r1' r2
+    | nil => nil
+  end.
+
+
+Eval simpl in project ((1 :: nil) :: (2 :: nil) :: nil) 0.
+
+Definition runQuery (q : Query) (inputRelation1 : relation) (inputRelation2 : relation) : option relation :=
   match q with 
   | Select b => match b with 
-                | BTrue => Some inputRelation
+                | BTrue => Some inputRelation1
                 | BFalse => Some nil
                 end
-  | SelectIf pr => Some (select pr inputRelation)
-  | Project index => project inputRelation index
+  | SelectIf pr => Some (select pr inputRelation1)
+  | Project index => project inputRelation1 index
+  | JoinFirst => Some (nljoin inputRelation1 inputRelation2)
   end.
+
+Eval compute in runQuery JoinFirst ((1::2::nil) :: (2::3::nil) :: nil) ((3::4::nil) :: (1::10::nil) :: (1::12::nil) :: nil).
 
 (**
   IMP syntax
@@ -107,7 +130,8 @@ Inductive BExp : Set :=
   | Pred1Exp : BExp. 
 
 Inductive Exp : Set :=
-  | InputRelation : Exp
+  | InputRelation1 : Exp
+  | InputRelation2 : Exp
   | RelationExp : relation -> Exp
 (*  | TupleExp : tuple -> Exp *)
   | NatExp : nat -> Exp
@@ -116,9 +140,10 @@ Inductive Exp : Set :=
 (* It turns out that Forall is already defined in Coq, so I used ForAll *)
 Inductive Statement : Set :=
   | Assign : VarName -> Exp -> Statement
-  | ForAll : VarName -> Statement -> Statement
+  | ForAll : VarName -> Exp -> Statement -> Statement
   | ProjectTuple : Exp -> VarName -> Statement
-  | SelectTuple : Exp -> VarName -> Statement.
+  | SelectTuple : Exp -> VarName -> Statement
+  | MatchTuples : VarName -> VarName -> Statement.
 
 Inductive ImpProgram : Set :=
   | Seq : Statement -> ImpProgram -> ImpProgram
@@ -131,14 +156,14 @@ Inductive ImpProgram : Set :=
 Definition queryToImp (q : Query) : option ImpProgram :=
   match q with
   | Select b => match b with
-                | BTrue => Some (Seq (Assign ResultName InputRelation) Skip) 
+                | BTrue => Some (Seq (Assign ResultName InputRelation1) Skip) 
                 | BFalse => Some (Seq (Assign ResultName (RelationExp nil)) Skip)   
                 end
   | Project index => Some 
                      (Seq 
                       (Assign ResultName (RelationExp nil))
                       (Seq
-                        (ForAll (IndexedVarName 0)
+                        (ForAll (IndexedVarName 0) InputRelation1
                           (ProjectTuple (NatExp index) (IndexedVarName 0)))
                         Skip))
   | SelectIf pr => match pr with
@@ -147,7 +172,7 @@ Definition queryToImp (q : Query) : option ImpProgram :=
                      (Seq 
                       (Assign ResultName (RelationExp nil))
                       (Seq
-                        (ForAll (IndexedVarName 0)
+                        (ForAll (IndexedVarName 0) InputRelation1
                           (SelectTuple (BoolExp (BoolBExp b)) (IndexedVarName 0)))
                         Skip))
                      | PredFirst1 =>
@@ -155,25 +180,33 @@ Definition queryToImp (q : Query) : option ImpProgram :=
                      (Seq 
                       (Assign ResultName (RelationExp nil))
                       (Seq
-                        (ForAll (IndexedVarName 0)
+                        (ForAll (IndexedVarName 0) InputRelation1
                           (SelectTuple (BoolExp Pred1Exp) (IndexedVarName 0)))
                         Skip))
                     end
+   | JoinFirst => Some
+                     (Seq
+                       (Assign ResultName (RelationExp nil))
+                       (Seq
+                         (ForAll (IndexedVarName 0) InputRelation1
+                           (ForAll (IndexedVarName 1) InputRelation2
+                             (MatchTuples (IndexedVarName 0) (IndexedVarName 1))))
+                         Skip))
 
                         
   end.
 
 (* heap is a tuple *)
-Fixpoint runStatement (s: Statement) (input: relation) (heap: tuple) : option relation :=
+Fixpoint runStatement (s: Statement) (input1: relation) (input2: relation) (heap: tuple * tuple) (nested: bool) : option relation :=
   match s with
   | Assign ResultName e => match e with
-                           | InputRelation => Some input
+                           | InputRelation1 => Some input1
                            | RelationExp rexp => Some rexp 
                            | _ => None
                            end
   | Assign _ _ => None
   | ProjectTuple (NatExp index) (IndexedVarName vnIndex) =>
-          match projectTuple heap index with
+          match projectTuple (fst heap) index with
           | Some tup => Some (tup :: nil)
           | None => None
           end
@@ -181,30 +214,35 @@ Fixpoint runStatement (s: Statement) (input: relation) (heap: tuple) : option re
   | SelectTuple (BoolExp bexp) (IndexedVarName vnIndex) =>
       match bexp with
         | BoolBExp b => match b with
-                          | BTrue => Some (heap :: nil)
+                          | BTrue => Some ((fst heap) :: nil)
                           | BFalse => Some nil
                         end
-        | Pred1Exp => match heap with
-                        | TCons 1 _ => Some (heap :: nil)
+        | Pred1Exp => match (fst heap) with
+                        | 1 :: _ => Some ((fst heap) :: nil)
                         | _ => Some nil
                       end
       end
   | SelectTuple _ _ => None
-  | ForAll (IndexedVarName index)  s' =>
-      let fix helper (rel: relation) :=
+  | ForAll (IndexedVarName index) _ s' =>
+      let fix helper (rel: relation) (nested' : bool) :=
         match rel with
         | nil => Some nil
         | t :: rem => 
-          match (runStatement s' input t) with
+          let heap' := if nested' then pair (fst heap) t else pair t nil in
+          match (runStatement s' input1 input2 heap' true) with
           | None => None
-          | Some res => match (helper rem) with
+          | Some res => match (helper rem nested') with
                         | Some rem' => Some (res ++ rem')
                         | None => None
                         end
           end
         end
-      in helper input
-  | ForAll _ _ => None
+      in if nested then helper input2 true else helper input1 false 
+  | ForAll _ _ _ => None
+  | MatchTuples (IndexedVarName vn1) (IndexedVarName vn2) =>
+       let (t1, t2) := ((fst heap), (snd heap)) in
+       if joineq t1 t2 then Some ((t1 ++ t2) :: nil) else Some nil
+  | MatchTuples _ _ => None
   end.
 
 
@@ -215,22 +253,23 @@ Fixpoint runStatement (s: Statement) (input: relation) (heap: tuple) : option re
    recursive. Special thanks go to Eric Mullen and Zach
    Tatlock.
 *)
-Definition runImp (p : ImpProgram) (input : relation) : option relation :=
+Definition runImp (p : ImpProgram) (input1 : relation) (input2 : relation) : option relation :=
   let fix helper (p : ImpProgram) (result: relation) : option relation := 
     match p with
     | Skip => Some result
-    | Seq s p' => match (runStatement s input TNil) with
+    | Seq s p' => match (runStatement s input1 input2 (pair nil nil) false) with
                     | Some res => helper p' (result ++ res)
                     | None => None
                   end
     end
   in helper p nil.
 
-Fixpoint runImp' (p: ImpProgram) (input: relation) : option relation :=
+
+Fixpoint runImp' (p: ImpProgram) (input1: relation) (input2 : relation) : option relation :=
   match p with
     | Skip => Some nil
-    | Seq s p' => match (runStatement s input TNil) with
-                    | Some res => match runImp' p' input with
+    | Seq s p' => match (runStatement s input1 input2 (pair nil nil) false) with
+                    | Some res => match runImp' p' input1 input2 with
                                     | Some remres => Some (res ++ remres)
                                     | None => None
                                       end
@@ -238,48 +277,55 @@ Fixpoint runImp' (p: ImpProgram) (input: relation) : option relation :=
                       end
 end.
 
+
 (** 
   Test cases
 **)
 Eval compute in let p := queryToImp (Project 0) in
                         match p with 
                           | None => None
-                          | Some p' => runImp p' ((TCons 1 (TCons 2 TNil)) :: (TCons 3 (TCons 4 TNil)) :: nil)
+                          | Some p' => runImp' p' ((1 :: 2 :: nil) :: (3 :: 4 :: nil) :: nil) nil
 end.
 (* = Some [(1),(3)] *)
 
 Eval compute in let p := queryToImp (Project 2) in
                         match p with 
                           | None => None
-                          | Some p' => runImp p' ((TCons 1 (TCons 2 TNil)) :: (TCons 3 (TCons 4 TNil)) :: nil)
+                          | Some p' => runImp' p' ((1 :: 2 :: nil) :: (3::4::nil) :: nil) nil
 end.
 (* = None *)
 
 Eval compute in let p := queryToImp (Project 1) in
                         match p with 
                           | None => None
-                          | Some p' => runImp p' ((TCons 1 (TCons 2 TNil)) :: (TCons 3 (TCons 4 TNil)) :: nil)
+                          | Some p' => runImp' p' ((1 :: 2 :: nil) :: (3::4::nil) :: nil) nil
 end.
 (* = Some [(2),(4)] *)
 
 Eval compute in let p := queryToImp (SelectIf (PredBool BTrue)) in
                           match p with
                             | None => None
-                            | Some p' => runImp p' ((TCons 1 (TCons 2 TNil)) :: (TCons 3 (TCons 4 TNil)) :: nil)
+                            | Some p' => runImp' p' ((1 :: 2 :: nil) :: (3::4::nil) :: nil) nil
 end.
 (* = Some [(1,2),(3,4)] *)
 
 Eval compute in let p := queryToImp (SelectIf (PredBool BFalse)) in
                           match p with
                             | None => None
-                            | Some p' => runImp p' ((TCons 1 (TCons 2 TNil)) :: (TCons 3 (TCons 4 TNil)) :: nil)
+                            | Some p' => runImp' p' ((1 :: 2 :: nil) :: (3::4::nil) :: nil) nil
 end.
 
 Eval compute in let p := queryToImp (SelectIf PredFirst1) in
                         match p with 
                           | None => None
-                          | Some p' => runImp p' ((TCons 1 (TCons 2 TNil)) :: (TCons 3 (TCons 4 TNil)) :: (TCons 0 (TCons 1 TNil)) :: (TCons 1 (TCons 6 TNil)) :: nil)
+                          | Some p' => runImp' p' ((1::2::nil) :: (3::4::nil) :: (0::1::nil) :: (1::6::nil) :: nil) nil
 end. 
+
+Eval compute in let p := queryToImp JoinFirst in
+  match p with
+    | None => None
+    | Some p' => runImp' p' ((1::2::nil) :: (2::3::nil) :: nil) ((3::4::nil) :: (1::10::nil) :: (1::12::nil) :: nil)
+end.
 (* = Some [(1,2),(1,6)] *)
 
 (**
@@ -291,11 +337,11 @@ it is possible if we rely on monotonic query processing *)
 
 Ltac inv H := inversion H; subst; clear H.
 Ltac unfold_all := repeat match goal with 
-                  | [ |- runImp' _ _ = _ ] => unfold runImp'; [repeat break_match; try discriminate]
-                  | [H: runImp' _ _ = _ |- _ ] => unfold runImp' in H; [repeat break_match; try discriminate]
-                  | [H: runQuery _ _ = _ |- _ ] => unfold runQuery in H; [repeat break_match; try discriminate]
+                  | [ |- runImp' _ _ _ = _ ] => unfold runImp'; [repeat break_match; try discriminate]
+                  | [H: runImp' _ _ _ = _ |- _ ] => unfold runImp' in H; [repeat break_match; try discriminate]
+                  | [H: runQuery _ _ _ = _ |- _ ] => unfold runQuery in H; [repeat break_match; try discriminate]
                   | H: project _ _ = _ |- _ => unfold project in H                 
-                  | [H: runStatement _ _ _ = _ |- _ ] => unfold runStatement in H; [repeat break_match; try discriminate]
+                  | [H: runStatement _ _ _ _ _ = _ |- _ ] => unfold runStatement in H; [repeat break_match; try discriminate]
                 end.
 Ltac inv_somes := repeat match goal with
                            | [ H: Some _ = Some _ |- _ ] => inv H
@@ -315,11 +361,15 @@ Lemma list_eq : forall (A : Type ) (h : A) t t' (h' : A), h :: t = h' :: t' -> (
 crush.
 Qed.
 
+Ltac massage_ihr1 := match goal with
+                              | H:context [ forall r2 _, runQuery _ _ _ = _ -> runImp' _ _ _ = _ ] |- _  => specialize (H r2); unfold runQuery in H
+                     end.
+
 Theorem queryEquivalence'': 
   forall (q : Query) (p : ImpProgram),
     queryToImp q = Some p ->
-      forall (r r' : relation), runQuery q r = Some r' ->
-        runImp' p r = Some r'. 
+      forall (r1 r2 r' : relation), runQuery q r1 r2 = Some r' ->
+        runImp' p r1 r2 = Some r'. 
   
 (* automagic!
   induction q; [
@@ -348,41 +398,45 @@ intros; destruct b; crush; f_equal; crush.
 
 (* Project case *)
 intros p Hc; inv Hc.
-induction r. crush. 
+induction r1. crush. 
 
   intros.
 
 unfold_all.
 f_equal.
-fold project in Heqo5.
-fold (runQuery (Project n) r) in Heqo5.
-apply IHr in Heqo5. clear IHr.       (* apply is smart, no need to specialize IHr's r'*)
+massage_ihr1.
+unfold project in IHr1.
+apply IHr1 in Heqo6. clear IHr1.
 unfold_all.
-rewrite Heqo8 in Heqo3. clear Heqo8.
-inv_somes.
-trivial.
-
-fold project in Heqo5.
-fold (runQuery (Project n) r) in Heqo5.
-apply IHr in Heqo5. clear IHr.
-unfold_all.
-inv_somes.
+rewrite Heqo9 in Heqo3. clear Heqo9.
+unfold fst in Heqo4.
 crush.
 
+fold project in Heqo6.
+massage_ihr1.
+apply IHr1 in Heqo6. clear IHr1.
+unfold_all.
+crush.
+
+fold project in Heqo5.      (* new case *)
+massage_ihr1.
+apply IHr1 in Heqo5. clear IHr1.
+unfold_all.
+crush.
 
 (* SelectIf case *)
 intros p0 Hc; inv Hc.
 destruct p.
-induction r; destruct b. crush. crush.
+induction r1; destruct b. crush. crush.
 
 inv H0.
 intros.
 
 unfold runQuery in H. simpl in H. inversion H. clear H.
 destruct r'. crush. inversion H1. subst a. clear H2.
-unfold runQuery in IHr.
-assert (Some (select (PredBool BTrue) r) = Some r'). crush.
-apply IHr in H. clear IHr.
+massage_ihr1.
+assert (Some (select (PredBool BTrue) r1) = Some r'). crush.
+apply IHr1 in H. clear IHr1.
 
 rewrite H1.
 
@@ -421,16 +475,17 @@ break_match; discriminate.
 intros.
 inv H0.
 unfold_all.
-unfold runQuery in IHr.
+massage_ihr1.
 unfold select in H. fold select in H. (* gets rid of "a" *)
-apply IHr in H. clear IHr.
+apply IHr1 in H. clear IHr1.
 unfold_all.
 rewrite Heqo5 in Heqo2.
 inv_somes.
 simpl. reflexivity.
 
 unfold select in H. fold select in H. (* gets rid of "a" *)
-apply IHr in H. clear IHr.
+massage_ihr1.
+apply IHr1 in H. clear IHr1.
 unfold_all.
 rewrite Heqo5 in Heqo2.
 inv_somes.
@@ -438,76 +493,61 @@ discriminate.
 
 
 (* SelectIf PredFirst1 *)
-induction r. crush.
+induction r1. crush.
 
 intros.
 inversion H0. clear H0.
 unfold runQuery in H.
 unfold select in H.
 break_match.
-break_match.
-unfold runQuery in IHr.
-unfold select in IHr.
-apply IHr in H. clear IHr.
+massage_ihr1. 
+apply IHr1 in H. clear IHr1.
 inversion H2 in H. clear H2 H0.
 unfold_all.
-rewrite Heqo4 in Heqo5. clear Heqo4.
-crush. 
+rewrite Heqo4 in Heqo6. clear Heqo4.
+crush.
 
-rewrite Heqo4 in Heqo5. clear Heqo4.
+rewrite Heqo4 in Heqo6. clear Heqo4.
 discriminate.
 
 break_match; try discriminate.
 unfold_all.
-unfold runQuery in IHr.
-unfold select in IHr.
-destruct r'.
+massage_ihr1.
+apply IHr1 in H. clear IHr1.
+inv H2. clear H0.
+unfold_all.
+rewrite Heqo3 in Heqo6. clear Heqo3.
 crush.
 
+massage_ihr1.
+apply IHr1 in H. clear IHr1.
+inv H2; clear H0.
+unfold_all.
+rewrite Heqo3 in Heqo6. clear Heqo3.
+discriminate.
+
+break_match; try discriminate.
+destruct r'.
+discriminate.
 apply some_list_eq in H.
-destruct H. fold select in H. fold select in IHr.
-apply some_eq in H.
-apply IHr in H. clear IHr.
+destruct H. 
+massage_ihr1.
+apply some_eq in H. 
+apply IHr1 in H. clear IHr1.
 inv H2. clear H1.
 unfold_all.
-rewrite Heqo2 in Heqo5. clear Heqo2.
-inv_somes. trivial.
+rewrite Heqo4 in Heqo6. clear Heqo4.
+crush.
 
-destruct r'. discriminate.
-fold select in H.
-apply some_list_eq in H.
-destruct H.
-unfold runQuery in IHr.
-apply some_eq in H.
-apply IHr in H. clear IHr.
-inv H2. clear H1.
-unfold_all.
-rewrite Heqo2 in Heqo5. clear Heqo2.
-discriminate.
+destruct r'; rewrite Heqo4 in Heqo6; clear Heqo4; crush.
 
-fold select in H.
-unfold runQuery in IHr.
-apply IHr in H. clear IHr.
+massage_ihr1.
+apply IHr1 in H. clear IHr1.
 inv H2. clear H0.
-unfold_all.
-rewrite Heqo4 in Heqo5. clear Heqo4.
-inv_somes. trivial.
+unfold_all; rewrite Heqo4 in Heqo6; clear Heqo4; crush.
 
-rewrite Heqo4 in Heqo5. clear Heqo4.
-discriminate.
 
-fold select in H.
-unfold runQuery in IHr.
-inv H2. clear H0.
-apply IHr in H. clear IHr.  (* applying IHr probably crushable if we first unfold_all inside IHr *)
-unfold_all.
-rewrite Heqo4 in Heqo5. clear Heqo4.
-inv_somes.
-trivial.
-
-rewrite Heqo4 in Heqo5. clear Heqo4.
-inv_somes.
-discriminate.
+(* Join first case *)
 Qed.
 (* wish list:
 - unify ProjectTuple and SelectTuple by bringing back AppendTuple
